\p
      طبق اتحاد پاسکال داریم:
     \[\binom{n+k}{k}+\binom{n+k}{k-1} = \binom{n+k+1}{k}\]
    از جمع تساوی‌های زیر که از اتحاد پاسکال به دست می‌آیند، می‌توان نتیجه مطلوب را گرفت:
    \[\binom{n}{0} = \binom{n+1}{0}\]
    \[\binom{n+1}{1} = \binom{n+2}{1}-\binom{n+1}{0}\]
    \[\binom{n+2}{2} = \binom{n+3}{2}-\binom{n+2}{1}\]
    \[\binom{n+3}{3} = \binom{n+4}{3}-\binom{n+3}{2}\]
    $$\vdots$$
    \[\binom{n+k}{k} = \binom{n+k+1}{k}-\binom{n+k}{k-1}\]
    \begin{center}
				$\rule{0.4\textwidth}{0.8pt}$
				\Huge{+}
	\end{center}
    $$\binom{n}{0}+\binom{n+1}{1}+\binom{n+2}{2}+\binom{n+3}{3}+...+\binom{n+k}{k} =$$
     $$\binom{n+k+1}{k}; k>0$$