\p
سمت چپ معادله برابر است با:
	$$\sum\limits_{k = 0}^m \frac{{m \choose k}}{{n \choose k}} = \sum\limits_{k = 0}^m \frac{\frac{m!}{k!(m - k)!}}{\frac{n!}{k!(n - k)!}} = \sum\limits_{k = 0}^m \frac{\frac{(n - k)!}{(n - m)!(m - k)!}}{\frac{n!}{(n - m)!m!}}$$
	
	$$= \sum\limits_{k = 0}^m \frac{{n - k \choose m - k}}{{n \choose m}} \mathrel{\overset{\makebox[0pt]{\mbox{\normalfont\tiny i = m - k}}}{=\joinrel=\joinrel=}} \frac{\sum\limits_{i = 0}^m {n - m + i \choose i}}{{n \choose m}} \mathrel{\overset{\makebox[0pt]{\text{\normalfont\tiny چوشی‌چی}}}{=\joinrel=\joinrel=}} \frac{{n+1 \choose m}}{{n \choose m}}$$
	
	$$= \frac{\frac{(n+1)!}{m!(n - m + 1)!}}{\frac{n!}{m!(n - m)!}} = \frac{n+1}{n - m + 1}$$
